work on the pointer compare rule

veric/SeparationLogic.v
@@ -77,6 +77,14 @@ Definition substopt {A} (ret: option ident) (v: environ -> val) (P: environ -> A
 Definition cast_expropt (e: option expr) t : environ -> option val :=
  match e with Some e' => `Some (eval_expr (Ecast e' t))  | None => `None end.
 
+Definition typecheck_tid_ptr_compare
+Delta id := 
+match (temp_types Delta) ! id with
+| Some (t, _) =>
+   is_int_type t 
+| None => false
+end. 
+
 Definition umapsto (sh: Share.t) (t: type) (v1 v2 : val): mpred :=
   match access_mode t with
   | By_value ch => 
@@ -371,6 +379,41 @@ Definition tc_expropt Delta (e: option expr) (t: type) : environ -> Prop :=
                      | Some e' => tc_expr Delta (Ecast e' t)
    end.
 
+Definition is_comparison op :=
+match op with 
+  | Cop.Oeq | Cop.One | Cop.Olt | Cop.Ogt | Cop.Ole | Cop.Oge => true              
+  | _ => false
+end. 
+
+Definition blocks_match op e1 e2  :=
+match op with Cop.Olt | Cop.Ogt | Cop.Ole | Cop.Oge => 
+  (fun rho =>
+  match (eval_expr e1 rho), (eval_expr e2 rho) with
+    Vptr b _, Vptr b2 _ => b=b2
+    | _, _ => False
+  end)
+| _ => fun rho => True
+end. 
+
+
+Definition cmp_ptr_no_mem e1 e2 c rho :=
+match eval_expr e1 rho, eval_expr e2 rho with
+Vptr b o, Vptr b1 o1 => 
+  if zeq b b1 then
+    Val.of_bool (Int.cmpu c o o1)
+  else
+    force_val (Cop.sem_cmp_mismatch c)
+| _, _ => Vundef
+end. 
+
+Definition op_to_cmp cop :=
+match cop with 
+| Cop.Oeq => Ceq | Cop.One =>  Cne
+| Cop.Olt => Clt | Cop.Ogt =>  Cgt 
+| Cop.Ole => Cle | Cop.Oge =>  Cge 
+| _ => Ceq (*doesn't matter*)
+end.
+
 Fixpoint arglist (n: positive) (tl: typelist) : list (ident*type) :=
  match tl with 
   | Tnil => nil
@@ -592,6 +635,25 @@ forall (Delta: tycontext) (P: environ->mpred) id e,
         (normal_ret_assert 
           (EX old:val, local (`eq (eval_id id) (subst id (`old) (eval_expr e))) &&
                             subst id (`old) P)).
+
+Axiom semax_ptr_compare : 
+forall {Espec: OracleKind},
+forall (Delta: tycontext) P id cmp e1 e2 ty sh1 sh2,
+    is_comparison cmp = true  ->
+   @semax Espec Delta 
+        ( |> (local (tc_expr Delta e1) &&
+             local (tc_expr Delta e2)  && 
+          local `(typecheck_tid_ptr_compare Delta id = true) &&  
+          local (blocks_match cmp e1 e2) &&
+          (`(mapsto_ sh1 (typeof e1)) (eval_expr e1 ) * TT) && 
+          (`(mapsto_ sh2 (typeof e2)) (eval_expr e2 ) * TT) && 
+          P))
+          (Sset id (Ebinop cmp e1 e2 ty)) 
+        (normal_ret_assert 
+          (EX old:val, 
+                 local (`eq (eval_id id)  (subst id `old 
+                     (cmp_ptr_no_mem e1 e2 (op_to_cmp cmp)))) &&
+                            subst id `old P)).
 
 Axiom semax_load : 
   forall {Espec: OracleKind},
