floyd/forward_lemmas.v
@@ -193,6 +193,51 @@ Qed.
 Hint Rewrite @closed_wrt_map_subst' using solve [auto with closed] : norm.
 Hint Rewrite @closed_wrt_map_subst' using solve [auto with closed] : subst.
 
+
+Lemma forward_ptr_compare_closed_now :
+forall Espec Delta P Q R id e1 e2 cmp ty sh1 sh2, 
+Forall (closed_wrt_vars (eq id)) Q ->
+Forall (closed_wrt_vars (eq id)) R ->
+closed_wrt_vars (eq id) ((cmp_ptr_no_mem e1 e2 
+                                    (op_to_cmp cmp))) ->
+PROPx P (LOCALx Q (SEPx R)) |-- (local (tc_expr Delta e1) && local (tc_expr Delta e2) &&
+      local `(typecheck_tid_ptr_compare Delta id = true) &&
+      local (blocks_match cmp e1 e2) &&
+      (`(mapsto_ sh1 (typeof e1)) (eval_expr e1) * TT) &&
+      (`(mapsto_ sh2 (typeof e2)) (eval_expr e2) * TT)) ->
+is_comparison cmp = true ->
+@semax Espec Delta
+  (PROPx P (LOCALx Q (SEPx R)))
+    (Sset id (Ebinop cmp e1 e2 ty))
+  ((normal_ret_assert
+     (EX  old : val,
+       PROPx P (LOCALx (`eq (eval_id id) 
+                     (cmp_ptr_no_mem e1 e2 
+                                    (op_to_cmp cmp)) :: Q)
+          (SEPx  R))))). 
+Proof. 
+intros. 
+eapply semax_pre_post; [ | | eapply (semax_ptr_compare Delta (PROPx P (LOCALx Q (SEPx R))) _ _ _ _ _ sh1 sh2)].
+eapply derives_trans; [ | apply now_later]. 
+intro rho. normalize. 
+apply andp_right; auto.
+specialize (H2 rho).   
+simpl in H2.
+normalize in H2. 
+normalize.
+ 
+intros ex vl rho.
+unfold normal_ret_assert. simpl. 
+repeat apply andp_right. 
+normalize. 
+normalize. 
+apply exp_right. apply Vundef. 
+normalize. 
+
+autorewrite with subst in *. normalize. 
+auto. 
+Qed. 
+
 Lemma forward_setx_closed_now':
   forall Espec Delta P (Q: list (environ -> Prop)) (R: list (environ->mpred)) id e,
   Forall (closed_wrt_vars (eq id)) Q ->
@@ -773,6 +818,64 @@ destruct (eval_expr e1 rho); simpl in *; try contradiction; auto.
 Qed.
 
 
+Lemma forward_ptr_compare': 
+forall Espec Delta P id e1 e2 sh1 sh2 cmp ty, 
+P |-- (local (tc_expr Delta e1) && local (tc_expr Delta e2) &&
+      local `(typecheck_tid_ptr_compare Delta id = true) &&
+      local (blocks_match cmp e1 e2) &&
+      (`(mapsto_ sh1 (typeof e1)) (eval_expr e1) * TT) &&
+      (`(mapsto_ sh2 (typeof e2)) (eval_expr e2) * TT)) ->
+is_comparison cmp = true ->
+@semax Espec Delta
+  P
+    (Sset id (Ebinop cmp e1 e2 ty))
+  ((normal_ret_assert
+     (EX  old : val,
+       (local (`eq (eval_id id) (subst id `old (cmp_ptr_no_mem e1 e2 
+                               (op_to_cmp cmp))))) &&
+       (subst id (`old)) P))).
+Proof. 
+intros.
+eapply semax_pre_post; [ | | apply (semax_ptr_compare Delta P _ _ _ _ _ sh1 sh2)].
+eapply derives_trans; [ | apply now_later]. 
+intro rho. normalize. 
+apply andp_right; auto.  
+eapply derives_trans. apply H. normalize. 
+intros ek vl rho. unfold normal_ret_assert. simpl. 
+normalize. 
+apply exp_right with x. normalize. 
+auto. 
+Qed. 
+
+Lemma forward_ptr_compare:
+forall Espec Delta P Q R id e1 e2 sh1 sh2 cmp ty, 
+PROPx P (LOCALx Q (SEPx R)) |-- (local (tc_expr Delta e1) && local (tc_expr Delta e2) &&
+      local `(typecheck_tid_ptr_compare Delta id = true) &&
+      local (blocks_match cmp e1 e2) &&
+      (`(mapsto_ sh1 (typeof e1)) (eval_expr e1) * TT) &&
+      (`(mapsto_ sh2 (typeof e2)) (eval_expr e2) * TT)) ->
+is_comparison cmp = true ->
+@semax Espec Delta
+  (PROPx P (LOCALx Q (SEPx R)))
+    (Sset id (Ebinop cmp e1 e2 ty))
+  ((normal_ret_assert
+     (EX  old : val,
+       PROPx P 
+        (LOCALx (`eq (eval_id id) 
+                     (subst id `old (cmp_ptr_no_mem e1 e2 
+                                    (op_to_cmp cmp))) ::
+                     map (subst id (`old)) Q)
+          (SEPx (map (subst id (`old)) R)))))). 
+Proof. 
+ intros.
+ eapply semax_post; [ | apply forward_ptr_compare' with (sh1 := sh1) (sh2 := sh2); auto].
+ intros.
+ autorewrite with ret_assert subst.
+ intro rho. simpl. normalize.
+ apply exp_right with x.
+ autorewrite with  subst. normalize.
+Qed. 
+
 Lemma forward_setx':
   forall Espec Delta P id e,
   (P |-- local (tc_expr Delta e) && local (tc_temp_id id (typeof e) Delta e) ) ->
@@ -794,6 +897,7 @@ intros ek vl rho; unfold normal_ret_assert. simpl; normalize.
 apply exp_right with x.
 normalize.
 Qed.
+
 
 Lemma forward_setx:
   forall Espec Delta P Q R id e,
